Add universe to fancy updates

spc/RobustIndexedInvariants.v
@@ -6,99 +6,101 @@ From iris Require base_logic.lib.invariants.
 Require Import Coqlib PCM PCMAux IProp IPM.
 Require Import Coq.Logic.ClassicalEpsilon.
 
-Local Notation index := nat.
-
+Local Notation universe := positive.
+Local Notation level := nat.
+  
 Section INDEXED_INVARIANT_SET.
 
   Context `{Σ : GRA.t}.
-  Context `{UNIV: Ensembles.Ensemble positive}.
 
-  Definition universe := { n : positive | Ensembles.In _ UNIV n }.
+  Class IInvSet (Vars : level -> Type) :=
+    { prop : forall (i : level), (Vars i) -> iProp }.
 
-  Class IInvSet (Vars : index -> Type) :=
-    { prop : forall (i : index), (Vars i) -> iProp }.
+  Definition InvSetRA (Vars : level -> Type) (n : level) : URA.t :=
+    (Auth.t (positive ==> URA.agree (Vars n)))%ra.
 
-  (* Class IInvIn {Vars : index -> Type} `{IInvSet Vars} (n : index) (P : iProp) := *)
-  (*   { inhabitant : Vars n *)
-  (*   ; inhabitant_eq : prop _ inhabitant = P *)
-  (*   }. *)
+  Definition IInvSetRA (Vars : level -> Type) : URA.t :=
+    URA.pointwise universe (@URA.pointwise_dep level (InvSetRA Vars)).
 
-  Definition InvSetRA (Vars : index -> Type) (n : index) : URA.t :=
-    (Auth.t (universe ==> URA.agree (Vars n)))%ra.
-
-  Definition IInvSetRA (Vars : index -> Type) : URA.t :=
-    @URA.pointwise_dep index (InvSetRA Vars).
-
-  Definition OwnEsRA : URA.t := URA.pointwise index CoPset.t.
-  Definition OwnDsRA : URA.t := URA.pointwise index (Auth.t Gset.t).
+  Definition OwnEsRA : URA.t :=
+    URA.pointwise universe (URA.pointwise level CoPset.t).
+  
+  Definition OwnDsRA : URA.t :=
+    URA.pointwise universe (URA.pointwise level (Auth.t Gset.t)).
 
 End INDEXED_INVARIANT_SET.
 
 Section PCM_OWN.
 
   Context `{Σ : GRA.t}.
-  Context `{UNIV: Ensembles.Ensemble positive}.
 
-  Definition OwnE `{@GRA.inG OwnEsRA Σ} (n : index) (E : coPset) :=
-    OwnM (@maps_to_res index CoPset.t n (Some E)).
+  Definition OwnE `{@GRA.inG OwnEsRA Σ} (u: universe) (n : level) (E : coPset) :=
+    OwnM (maps_to_res u (@maps_to_res level CoPset.t n (Some E))).
 
-  Definition OwnD `{@GRA.inG OwnDsRA Σ} (n : index) (D : gset positive) :=
-    OwnM (@maps_to_res index (Auth.t Gset.t) n (Auth.white (Some D : Gset.t))).
+  Definition OwnD `{@GRA.inG OwnDsRA Σ} (u: universe) (n : level) (D : gset positive) :=
+    OwnM (maps_to_res u (@maps_to_res level (Auth.t Gset.t) n (Auth.white (Some D : Gset.t)))).
 
-  Definition OwnD_auth `{@GRA.inG OwnDsRA Σ} (n : index) :=
-    (∃ D, OwnM (@maps_to_res index (Auth.t Gset.t) n (Auth.black (Some D : Gset.t))))%I.
+  Definition OwnD_auth `{@GRA.inG OwnDsRA Σ} (u: universe) (n : level) :=
+    (∃ D, OwnM (maps_to_res u (@maps_to_res level (Auth.t Gset.t) n (Auth.black (Some D : Gset.t)))))%I.
 
-  Definition OwnI_white {Vars} (n : index) (i : positive) (p : Vars n) : IInvSetRA Vars :=
-    @maps_to_res_dep index (InvSetRA Vars)
+  Definition OwnI_white {Vars} (u: universe) (n : level) (i : positive) (p : Vars n) : IInvSetRA Vars :=
+    maps_to_res u (
+    @maps_to_res_dep level (@InvSetRA Vars)
                      n
-                     (Auth.white (@maps_to_res positive (URA.agree (Vars n)) i (Some (Some p)))).
+                     (Auth.white (@maps_to_res positive (URA.agree (Vars n)) i (Some (Some p))))).
 
-  Definition OwnI {Vars} `{@GRA.inG (IInvSetRA Vars) Σ} (n : index) (i : positive) (p : Vars n) :=
-    OwnM (OwnI_white n i p).
+  Definition OwnI {Vars} `{@GRA.inG (IInvSetRA Vars) Σ} (u: universe) (n : level) (i : positive) (p : Vars n) :=
+    OwnM (OwnI_white u n i p).
 
-  Lemma OwnE_index_diff `{@GRA.inG OwnEsRA Σ} n1 n2 (E : coPset) :
-    (E <> ∅) -> OwnE n1 E ∗ OwnE n2 E ⊢ ⌜n1 <> n2⌝.
+  Lemma OwnE_level_diff `{@GRA.inG OwnEsRA Σ} u n1 n2 (E : coPset) :
+    (E <> ∅) -> OwnE u n1 E ∗ OwnE u n2 E ⊢ ⌜n1 <> n2⌝.
   Proof.
     intros NEMP.
     iIntros "[H1 H2]". iCombine "H1 H2" as "H". iPoseProof (OwnM_valid with "H") as "%WF".
-    iPureIntro. unfold maps_to_res in WF. rewrite /URA.wf /URA.add in WF. unseal "ra".
-    ss. intros EQ. subst n2. specialize (WF n1). des_ifs.
+    iPureIntro. intros EQ. subst n2.
+    rewrite /URA.wf /URA.add in WF. unseal "ra". ss. specialize (WF u).
+    rewrite /URA.wf /URA.add in WF. unseal "ra". ss. specialize (WF n1).
+    unfold maps_to_res in WF. des_ifs.
     rewrite /URA.wf /URA.add in WF. unseal "ra". ss. des_ifs. set_solver.
   Qed.
 
-  Lemma OwnE_exploit `{@GRA.inG OwnEsRA Σ} n (E1 E2 : coPset) :
-    OwnE n E1 ∗ OwnE n E2 ⊢ ⌜E1 ## E2⌝.
+  Lemma OwnE_exploit `{@GRA.inG OwnEsRA Σ} u n (E1 E2 : coPset) :
+    OwnE u n E1 ∗ OwnE u n E2 ⊢ ⌜E1 ## E2⌝.
   Proof.
     iIntros "[H1 H2]". iCombine "H1 H2" as "H". iPoseProof (OwnM_valid with "H") as "%WF".
-    iPureIntro. rewrite /URA.wf /URA.add in WF. unseal "ra". ss.
-    specialize (WF n). unfold maps_to_res in WF. des_ifs.
+    iPureIntro.
+    rewrite /URA.wf /URA.add in WF. unseal "ra". ss. specialize (WF u).
+    rewrite /URA.wf /URA.add in WF. unseal "ra". ss. specialize (WF n).
+    unfold maps_to_res in WF. des_ifs.
     rewrite /URA.wf /URA.add in WF. unseal "ra". ss; des_ifs.
   Qed.
 
-  Lemma OwnE_union `{@GRA.inG OwnEsRA Σ} n (E1 E2 : coPset) :
-    OwnE n E1 ∗ OwnE n E2 ⊢ OwnE n (E1 ∪ E2).
+  Lemma OwnE_union `{@GRA.inG OwnEsRA Σ} u n (E1 E2 : coPset) :
+    OwnE u n E1 ∗ OwnE u n E2 ⊢ OwnE u n (E1 ∪ E2).
   Proof.
     iIntros "H". iPoseProof (OwnE_exploit with "H") as "%D".
     iRevert "H". iApply from_sep. eapply from_sep_ownM.
-    unfold IsOp, maps_to_res, URA.add. ss. extensionalities k. unseal "ra".
-    des_ifs; ss.
-    - unfold URA.add. unseal "ra". ss. des_ifs.
+    unfold IsOp, maps_to_res, URA.add. ss. unseal "ra".
+    extensionalities u' n'. des_ifs; ss.
+    - repeat (unfold URA.add; unseal "ra"; ss; des_ifs).
+    - unfold URA.add. unseal "ra". ss. des_ifs. r_solve.
     - rewrite URA.unit_id. auto.
   Qed.
 
-  Lemma OwnE_disjoint `{@GRA.inG OwnEsRA Σ} n (E1 E2 : coPset) :
-    E1 ## E2 -> OwnE n (E1 ∪ E2) ⊢ OwnE n E1 ∗ OwnE n E2.
+  Lemma OwnE_disjoint `{@GRA.inG OwnEsRA Σ} u n (E1 E2 : coPset) :
+    E1 ## E2 -> OwnE u n (E1 ∪ E2) ⊢ OwnE u n E1 ∗ OwnE u n E2.
   Proof.
     i. unfold OwnE.
     iApply into_sep. eapply into_sep_ownM.
-    unfold IsOp, maps_to_res, URA.add. unseal "ra". ss.
-    extensionalities k. des_ifs.
-    - unfold URA.add. unseal "ra". ss. des_ifs.
+    unfold IsOp, maps_to_res, URA.add. ss. unseal "ra".
+    extensionalities u' n'. des_ifs.
+    - repeat (unfold URA.add; unseal "ra"; ss; des_ifs).
+    - unfold URA.add. unseal "ra". ss. des_ifs. r_solve.
     - rewrite URA.unit_id. auto.
   Qed.
 
-  Lemma OwnE_subset `{@GRA.inG OwnEsRA Σ} n (E1 E2 : coPset) :
-    E1 ⊆ E2 -> OwnE n E2 ⊢ OwnE n E1 ∗ (OwnE n E1 -∗ OwnE n E2).
+  Lemma OwnE_subset `{@GRA.inG OwnEsRA Σ} u n (E1 E2 : coPset) :
+    E1 ⊆ E2 -> OwnE u n E2 ⊢ OwnE u n E1 ∗ (OwnE u n E1 -∗ OwnE u n E2).
   Proof.
     iIntros (SUB) "E".
     assert (E2 = E1 ∪ E2 ∖ E1) as EQ.
@@ -110,14 +112,14 @@ Section PCM_OWN.
   Qed.
 
   Global Instance OwnI_persistent {Vars} `{@GRA.inG (IInvSetRA Vars) Σ}
-    n i p : Persistent (OwnI n i p).
+    u n i p : Persistent (OwnI u n i p).
   Proof.
     unfold OwnI, OwnI_white.
-    remember (@maps_to_res_dep index (InvSetRA Vars) n (Auth.white (@maps_to_res positive (URA.agree (Vars n)) i (Some (Some p))))) as r.
+    remember (@maps_to_res_dep level (InvSetRA Vars) n (Auth.white (@maps_to_res positive (URA.agree (Vars n)) i (Some (Some p))))) as r.
     unfold Persistent. iIntros "H".
     iPoseProof (@OwnM_persistently _ _ H _ with "H") as "#HP". iModIntro.
-    replace r with (URA.core r) at 2; auto.
-    subst. unfold maps_to_res_dep, maps_to_res. ss. extensionalities k. des_ifs.
+    replace (maps_to_res u r) with (URA.core (maps_to_res u r)) at 2. auto.
+    subst. unfold maps_to_res_dep, maps_to_res. ss. extensionalities u' n'. des_ifs.
   Qed.
 
 End PCM_OWN.
@@ -125,44 +127,45 @@ End PCM_OWN.
 Section WORLD_SATISFACTION.
 
   Context `{Σ : GRA.t}.
-  Context `{Vars : index -> Type}.
+  Context `{Vars : level -> Type}.
   Context `{@IInvSet Σ Vars}.
   Context `{@GRA.inG OwnEsRA Σ}.
   Context `{@GRA.inG OwnDsRA Σ}.
   Context `{@GRA.inG (IInvSetRA Vars) Σ}.
 
-  Variable n : index.
+  Variable u : universe.
+  Variable n : level.
   Local Notation Var := (Vars n).
 
   Definition inv_auth_black (I : gmap positive Var) : IInvSetRA Vars :=
-    @maps_to_res_dep index _
+    maps_to_res u (
+    @maps_to_res_dep level _
                      n (@Auth.black (positive ==> URA.agree Var)%ra
-                                    (fun (i : positive) => Some <$> (I !! i))).
+                                    (fun (i : positive) => Some <$> (I !! i)))).
 
   Definition inv_auth (I : gmap positive Var) := OwnM (inv_auth_black I).
 
   Definition inv_satall (I : gmap positive Var) :=
-    ([∗ map] i ↦ p ∈ I, (prop n p) ∗ OwnD n {[i]} ∨ OwnE n {[i]})%I.
+    ([∗ map] i ↦ p ∈ I, (prop n p) ∗ OwnD u n {[i]} ∨ OwnE u n {[i]})%I.
 
-  Definition wsat : iProp := (OwnD_auth n ∗ ∃ I, inv_auth I ∗ inv_satall I)%I.
-
+  Definition wsat : iProp := (OwnD_auth u n ∗ ∃ I, inv_auth I ∗ inv_satall I)%I.
 
   Lemma alloc_name φ
-        (INF : forall (E : index -> option (gset positive)) n,
+        (INF : forall (E : level -> option (gset positive)) n,
             match E n with
             | None => True
             | Some G => (exists i, i ∉ G /\ φ i)
             end)
-    : OwnD_auth n ⊢ #=> OwnD_auth n ∗ ∃ i, ⌜φ i⌝ ∧ OwnD n {[i]}.
+    : OwnD_auth u n ⊢ |==> OwnD_auth u n ∗ ∃ i, ⌜φ i⌝ ∧ OwnD u n {[i]}.
   Proof.
     iIntros "[% DA]". specialize (INF (fun _ => Some D) n). ss. des.
     assert (@URA.updatable
               OwnDsRA
-              (maps_to_res n (Auth.black (Some D : Gset.t)))
-              ((maps_to_res n (Auth.black (Some (D ∪ {[i]}) : Gset.t)))
+              (maps_to_res u (maps_to_res n (Auth.black (Some D : Gset.t))))
+              ((maps_to_res u (maps_to_res n (Auth.black (Some (D ∪ {[i]}) : Gset.t))))
                  ⋅
-                 (maps_to_res n (Auth.white (Some {[i]} : Gset.t))))) as UPD.
-    { rewrite maps_to_res_add. apply maps_to_updatable.
+                 (maps_to_res u (maps_to_res n (Auth.white (Some {[i]} : Gset.t)))))) as UPD.
+    { rewrite !maps_to_res_add. do 2 apply maps_to_res_updatable.
       ii. ur in H3. des_ifs. des. rewrite URA.unit_idl in H3.
       unfold URA.extends in H3. des. ur in H3.
       ur. rewrite URA.unit_idl. split.
@@ -181,12 +184,12 @@ Section WORLD_SATISFACTION.
   Qed.
 
   Lemma wsat_OwnI_alloc_gen p φ
-        (INF : forall (E : index -> option (gset positive)) n,
+        (INF : forall (E : level -> option (gset positive)) n,
             match E n with
             | None => True
             | Some G => (exists i, i ∉ G /\ φ i)
             end)
-    : wsat ⊢ #=> (∃ i, ⌜φ i⌝ ∧ OwnI n i p) ∗ (prop n p -∗ wsat).
+    : wsat ⊢ |==> (∃ i, ⌜φ i⌝ ∧ OwnI u n i p) ∗ (prop n p -∗ wsat).
   Proof.
     iIntros "[DA [% [AUTH SAT]]]".
     iMod (alloc_name (fun i => i ∉ dom I /\ φ i) with "DA") as "[DA [% [[%iI %iφ] D]]]".
@@ -200,11 +203,12 @@ Section WORLD_SATISFACTION.
     pose (<[i:=p]> I) as I'.
 
     assert (URA.updatable
-              (maps_to_res_dep n (@Auth.black (positive ==> URA.agree Var)%ra (fun i => Some <$> (I !! i))) : IInvSetRA Vars)
-              ((maps_to_res_dep n (@Auth.black (positive ==> URA.agree Var)%ra (fun i => Some <$> (I' !! i))) : IInvSetRA Vars)
-                 ⋅
-                 (maps_to_res_dep n (Auth.white (@maps_to_res _ (URA.agree Var) i (Some (Some p)))) : IInvSetRA Vars))).
-    { setoid_rewrite maps_to_res_dep_add. apply maps_to_res_dep_updatable.
+              (maps_to_res u (maps_to_res_dep n (@Auth.black (positive ==> URA.agree Var)%ra (fun i => Some <$> (I !! i)))): IInvSetRA Vars)
+              ((maps_to_res u (maps_to_res_dep n (@Auth.black (positive ==> URA.agree Var)%ra (fun i => Some <$> (I' !! i)))): IInvSetRA Vars)
+               ⋅
+               (maps_to_res u (maps_to_res_dep n (Auth.white (@maps_to_res _ (URA.agree Var) i (Some (Some p))))): IInvSetRA Vars))).
+    { setoid_rewrite maps_to_res_add. setoid_rewrite maps_to_res_dep_add.
+      apply maps_to_res_updatable. apply maps_to_res_dep_updatable.
       apply Auth.auth_alloc. ii. des. rewrite URA.unit_idl in FRAME. subst. split.
       { rr; unseal "ra". ss. intro. rr; unseal "ra". destruct (I' !! k); ss. }
       rr. subst I'.
@@ -227,28 +231,30 @@ Section WORLD_SATISFACTION.
   Qed.
 
   Lemma wsat_OwnI_alloc p φ
-        (INF : forall (E : index -> option (gset positive)) n,
+        (INF : forall (E : level -> option (gset positive)) n,
             match E n with
             | None => True
             | Some G => (exists i, i ∉ G /\ φ i)
             end)
-    : wsat ∗ prop n p ⊢ #=> (∃ i, ⌜φ i⌝ ∧ OwnI n i p) ∗ wsat.
+    : wsat ∗ prop n p ⊢ |==> (∃ i, ⌜φ i⌝ ∧ OwnI u n i p) ∗ wsat.
   Proof.
     iIntros "[W P]".
-    iMod (wsat_OwnI_alloc_gen with "W") as "[I W]"; eauto.
+    iMod (wsat_OwnI_alloc_gen with "W") as "[I W]". eauto.
     iFrame. iModIntro. iApply "W". iFrame.
   Qed.
 
   Lemma wsat_OwnI_open i p :
-    OwnI n i p ∗ wsat ∗ OwnE n {[i]} ⊢ #=> prop n p ∗ wsat ∗ OwnD n {[i]}.
+    OwnI u n i p ∗ wsat ∗ OwnE u n {[i]} ⊢ |==> prop n p ∗ wsat ∗ OwnD u n {[i]}.
   Proof.
     iIntros "(I & [DA [% [AUTH SAT]]] & EN)". iModIntro.
     unfold OwnI, inv_auth, inv_satall.
     iCombine "AUTH I" as "AUTH".
     iPoseProof (OwnM_valid with "AUTH") as "%WF".
     assert (Hip : I !! i = Some p).
-    { unfold inv_auth_black, OwnI_white in WF. setoid_rewrite maps_to_res_dep_add in WF.
-      unfold maps_to_res_dep, maps_to_res in WF. apply (pwd_lookup_wf _ n) in WF. ss. des_ifs.
+    { unfold inv_auth_black, OwnI_white in WF.
+      setoid_rewrite maps_to_res_add in WF. setoid_rewrite maps_to_res_dep_add in WF.
+      unfold maps_to_res_dep, maps_to_res in WF.
+      apply (pw_lookup_wf _ u) in WF. apply (pwd_lookup_wf _ n) in WF. ss. des_ifs.
       unfold eq_rect_r in WF. rewrite <- Eqdep.EqdepTheory.eq_rect_eq in WF.
       apply Auth.auth_included in WF. rename WF into EXTENDS.
       apply pw_extends in EXTENDS. specialize (EXTENDS i).
@@ -262,6 +268,7 @@ Section WORLD_SATISFACTION.
     iPoseProof (big_sepM_delete _ _ _ _ Hip with "SAT") as "[[[H1 H2]|H1] SAT]".
     2: { iCombine "EN H1" as "F". iPoseProof (OwnM_valid with "F") as "%WF".
          exfalso. unfold maps_to_res, URA.wf, URA.add in WF. unseal "ra". ss.
+         specialize (WF u). unfold URA.wf, URA.add in WF. unseal "ra". ss.
          specialize (WF n). des_ifs. unfold URA.wf, URA.add in WF. unseal "ra".
          ss. des_ifs. set_solver.
     }
@@ -270,15 +277,17 @@ Section WORLD_SATISFACTION.
   Qed.
 
   Lemma wsat_OwnI_close i p :
-    OwnI n i p ∗ wsat ∗ prop n p ∗ OwnD n {[i]} ⊢ #=> wsat ∗ OwnE n {[i]}.
+    OwnI u n i p ∗ wsat ∗ prop n p ∗ OwnD u n {[i]} ⊢ |==> wsat ∗ OwnE u n {[i]}.
   Proof.
     iIntros "(I & [DA [% [AUTH SAT]]] & P & DIS)". iModIntro.
     unfold OwnI, inv_auth, inv_satall.
     iCombine "AUTH I" as "AUTH".
     iPoseProof (OwnM_valid with "AUTH") as "%WF".
     assert (Hip : I !! i = Some p).
-    { unfold inv_auth_black, OwnI_white in WF. setoid_rewrite maps_to_res_dep_add in WF.
-      unfold maps_to_res_dep, maps_to_res in WF. apply (pwd_lookup_wf _ n) in WF. ss. des_ifs.
+    { unfold inv_auth_black, OwnI_white in WF.
+      setoid_rewrite maps_to_res_add in WF. setoid_rewrite maps_to_res_dep_add in WF.
+      unfold maps_to_res_dep, maps_to_res in WF.
+      apply (pw_lookup_wf _ u) in WF. apply (pwd_lookup_wf _ n) in WF. ss. des_ifs.
       unfold eq_rect_r in WF. rewrite <- Eqdep.EqdepTheory.eq_rect_eq in WF.
       apply Auth.auth_included in WF. rename WF into EXTENDS.
       apply pw_extends in EXTENDS. specialize (EXTENDS i).
@@ -293,6 +302,7 @@ Section WORLD_SATISFACTION.
     iPoseProof (big_sepM_delete _ _ _ _ Hip with "SAT") as "[[[H1 H2]|H1] SAT]".
     { iCombine "DIS H2" as "F". iPoseProof (OwnM_valid with "F") as "%WF".
       exfalso. unfold maps_to_res, URA.wf, URA.add in WF. unseal "ra". ss.
+      specialize (WF u). unfold URA.wf, URA.add in WF. unseal "ra". ss.
       specialize (WF n). des_ifs.
       unfold URA.wf, URA.add in WF. unseal "ra". ss.
       ur in WF. des_ifs. set_solver.
@@ -302,10 +312,10 @@ Section WORLD_SATISFACTION.
   Qed.
 
   Lemma wsat_init :
-    OwnM (maps_to_res n (Auth.black (Some ∅ : Gset.t)) : OwnDsRA)
-         ∗
-         OwnM (maps_to_res_dep n (@Auth.black (positive ==> URA.agree Var)%ra (fun (i : positive) => None)) : IInvSetRA _)
-         ⊢ wsat.
+    OwnM (maps_to_res u (maps_to_res n (Auth.black (Some ∅ : Gset.t))) : OwnDsRA)
+    ∗
+    OwnM (maps_to_res u (maps_to_res_dep n (@Auth.black (positive ==> URA.agree Var)%ra (fun (i : positive) => None))) : IInvSetRA _)
+    ⊢ wsat.
   Proof.
     iIntros "[H1 H2]". iSplitL "H1".
     { iExists ∅. iFrame. }
@@ -314,73 +324,143 @@ Section WORLD_SATISFACTION.
 
 End WORLD_SATISFACTION.
 
+Section POSITIVE_AUX.
+
+  Fixpoint pos_sup (p i: positive) : bool :=
+    match p, i with
+    | 1, _ => true
+    | p'~0, i'~0 => pos_sup p' i'
+    | p'~1, i'~1 => pos_sup p' i'
+    | _, _ => false
+    end%positive.
+
+  Fixpoint pos_ext_0 (p: positive) : positive :=
+    match p with
+    | 1 => 1~0
+    | p'~0 => (pos_ext_0 p')~0
+    | p'~1 => (pos_ext_0 p')~1
+    end%positive.
+
+  Fixpoint pos_ext_1 (p: positive) : positive :=
+    match p with
+    | 1 => 1~1
+    | p'~0 => (pos_ext_1 p')~0
+    | p'~1 => (pos_ext_1 p')~1
+    end%positive.
+
+  Lemma pos_ext_0_sup p:
+    pos_sup p (pos_ext_0 p).
+  Proof. induction p; s; eauto. Qed.
+
+  Lemma pos_ext_1_sup p:
+    pos_sup p (pos_ext_1 p).
+  Proof. induction p; s; eauto. Qed.
+
+  Lemma pos_sup_refl p:
+    pos_sup p p.
+  Proof. induction p; s; eauto. Qed.
+  
+  Lemma pos_sup_trans p0 p1 p2
+    (EXT1: pos_sup p0 p1)
+    (EXT2: pos_sup p1 p2)
+    :
+    pos_sup p0 p2.
+  Proof.
+    revert_until p0. induction p0; i; destruct p1, p2; ss; eauto.
+  Qed.
+  
+End POSITIVE_AUX.
+
 Section WSATS.
 
   Context `{Σ : GRA.t}.
-  Context `{Vars : index -> Type}.
+  Context `{Vars : level -> Type}.
   Context `{@IInvSet Σ Vars}.
   Context `{@GRA.inG OwnEsRA Σ}.
   Context `{@GRA.inG OwnDsRA Σ}.
   Context `{@GRA.inG (IInvSetRA Vars) Σ}.
 
-  Definition OwnDs_auth_black (x : index) : OwnDsRA :=
-    (fun n => if (lt_dec n x)
-           then ε
-           else Auth.black (Some ∅ : Gset.t)).
+  Definition OwnDs_auth_black (u: universe) (n : level) : OwnDsRA :=
+    (fun u' n' =>
+       if (u' =? u)%positive
+       then
+         (if (lt_dec n' n)
+          then ε
+          else Auth.black (Some ∅ : Gset.t))
+       else
+         (if (pos_sup u u')
+          then Auth.black (Some ∅ : Gset.t)
+          else ε)).
 
-  Definition OwnDs_auth (x : index) := OwnM (OwnDs_auth_black x).
+  Definition wsats_auth_black u n : IInvSetRA Vars :=
+    (fun u' n' =>
+       if (u' =? u)%positive
+       then
+         (if (lt_dec n' n)
+          then ε
+          else @Auth.black (positive ==> URA.agree (Vars n'))%ra (fun _ => None))
+       else
+         (if (pos_sup u u')
+          then @Auth.black (positive ==> URA.agree (Vars n'))%ra (fun _ => None)
+          else ε)).
 
-  Definition wsat_auth_black (x : index) : IInvSetRA Vars :=
-    (fun n => if (lt_dec n x)
-           then ε
-           else @Auth.black (positive ==> URA.agree (Vars n))%ra (fun _ => None)).
+  Definition wsats_auth u n :=
+    OwnM (OwnDs_auth_black u n) ** OwnM (wsats_auth_black u n).
 
-  Definition wsat_auth (x : index) := OwnM (wsat_auth_black x).
+  Definition wsats u n : iProp :=
+    ([∗ list] n' ∈ (seq 0 n), wsat u n')%I.
 
-  (* wsat n for all n < x *)
-  Definition wsats (x : index) := ([∗ list] n ∈ (seq 0 x), wsat n)%I.
-
-  Lemma unfold_wsats x :
-    wsats (S x) ⊢ (wsats x ∗ wsat x)%I.
+  Lemma unfold_wsats u n :
+    wsats u (S n) ⊢ (wsats u n ∗ wsat u n)%I.
   Proof.
-    iIntros "A". unfold wsats. replace (seq 0 (S x)) with (seq 0 x ++ [x]).
+    iIntros "A". unfold wsats. replace (seq 0 (S n)) with (seq 0 n ++ [n]).
     2:{ rewrite seq_S. ss. }
     iPoseProof (big_sepL_app with "A") as "[A [B C]]". ss. iFrame.
   Qed.
 
-  Lemma fold_wsats x :
-    (wsats x ∗ wsat x)%I ⊢ wsats (S x).
+  Lemma fold_wsats u n :
+    (wsats u n ∗ wsat u n)%I ⊢ wsats u (S n).
   Proof.
-    iIntros "A". unfold wsats. replace (seq 0 (S x)) with (seq 0 x ++ [x]).
+    iIntros "A". unfold wsats. replace (seq 0 (S n)) with (seq 0 n ++ [n]).
     2:{ rewrite seq_S. ss. }
     iApply big_sepL_app. ss. iDestruct "A" as "[A B]". iFrame.
   Qed.
 
-
-
   Lemma wsats_init_zero :
-    OwnM ((fun n => @Auth.black (positive ==> URA.agree (Vars n))%ra (fun _ => None)) : IInvSetRA Vars)
-         ⊢ wsat_auth 0 ∗ wsats 0.
+    OwnM ((fun u n => Auth.black (Some ∅ : Gset.t)) : OwnDsRA)
+    **
+    OwnM ((fun u n => @Auth.black (positive ==> URA.agree (Vars n))%ra (fun _ => None)) : IInvSetRA Vars)
+    ⊢ wsats_auth 1 0 ∗ wsats 1 0.
   Proof.
-    iIntros "H". iFrame. unfold wsats. ss.
+    iIntros "H". unfold wsats_auth, wsats. ss.
+    iSplitL; eauto. eapply eq_ind; [iApply "H"|].
+    f_equal; f_equal; extensionalities u n;
+      unfold OwnDs_auth_black, wsats_auth_black; destruct (u =? 1)%positive; ss.
   Qed.
 
-  Lemma wsat_auth_nin (x n : index) (NIN : x < n)
-    : OwnDs_auth x ∗ wsat_auth x
-                 ⊢ OwnDs_auth n ∗ wsat_auth n ∗ ([∗ list] m ∈ (seq x (n - x)), wsat m).
+  Lemma wsats_auth_nin u (n n' : level) (NIN : n < n')
+    : wsats_auth u n ⊢ wsats_auth u n' ∗
+                       ([∗ list] m ∈ (seq n (n' - n)), wsat u m).
   Proof.
     induction NIN.
-    - iIntros "[DA AUTH]". rename x into n. remember (S n) as x.
-      assert ((wsat_auth_black n) =
-                ((wsat_auth_black x)
-                   ⋅
-                   (maps_to_res_dep n (@Auth.black (positive ==> URA.agree (Vars n))%ra (fun (i : positive) => None))))).
-      { subst. extensionalities a. unfold wsat_auth_black, maps_to_res_dep.
-        unfold URA.add. unseal "ra". ss.
-        destruct (excluded_middle_informative (a = n)).
-        - subst a. des_ifs; try lia.
-          unfold eq_rect_r. ss. rewrite URA.unit_idl. reflexivity.
-        - destruct (le_dec a (S n)).
+    - iIntros "[DA AUTH]".
+      assert ((wsats_auth_black u n) =
+              ((wsats_auth_black u (S n))
+              ⋅
+              (maps_to_res u (maps_to_res_dep n (@Auth.black (positive ==> URA.agree (Vars n))%ra (fun (i : positive) => None)))))).
+      { subst. extensionalities u' n'. unfold wsats_auth_black, maps_to_res, maps_to_res_dep.
+        do 2 (unfold URA.add; unseal "ra"; ss).
+        destruct (u' =? u)%positive eqn: EQ; cycle 1.
+        { apply Pos.eqb_neq in EQ.
+          destruct (excluded_middle_informative (u' = u)); ss.
+          setoid_rewrite URA.unit_id. eauto.
+        }
+        apply Pos.eqb_eq in EQ. subst.
+        destruct (excluded_middle_informative (u=u)); ss.
+        destruct (excluded_middle_informative (n' = n)).
+        - subst. des_ifs; try lia.
+          unfold eq_rect_r. ss. r_solve.
+        - destruct (le_dec n' (S n)).
           { des_ifs; try lia.
             - rewrite URA.unit_idl. reflexivity.
             - rewrite URA.unit_id. reflexivity.
@@ -389,16 +469,23 @@ Section WSATS.
             rewrite URA.unit_id. reflexivity.
           }
       }
-      assert ((OwnDs_auth_black n) =
-                ((OwnDs_auth_black x)
-                   ⋅
-                   (maps_to_res n (Auth.black (Some ∅ : Gset.t))))).
-      { subst. extensionalities a. unfold OwnDs_auth_black, maps_to_res.
-        unfold URA.add. unseal "ra". ss.
-        destruct (excluded_middle_informative (a = n)).
-        - subst a. des_ifs; try lia.
+      assert ((OwnDs_auth_black u n) =
+              ((OwnDs_auth_black u (S n))
+              ⋅
+              (maps_to_res u (maps_to_res n (Auth.black (Some ∅ : Gset.t)))))).
+      { subst. extensionalities u' n'. unfold OwnDs_auth_black, maps_to_res.
+        do 2 (unfold URA.add; unseal "ra"; ss).
+        destruct (u' =? u)%positive eqn: EQ; cycle 1.
+        { apply Pos.eqb_neq in EQ.
+          destruct (excluded_middle_informative (u' = u)); ss.
+          setoid_rewrite URA.unit_id. eauto.
+        }
+        apply Pos.eqb_eq in EQ. subst.
+        destruct (excluded_middle_informative (u=u)); ss.
+        destruct (excluded_middle_informative (n' = n)).
+        - subst n'. des_ifs; try lia.
           unfold eq_rect_r. ss. rewrite URA.unit_idl. reflexivity.
-        - destruct (le_dec a (S n)).
+        - destruct (le_dec n' (S n)).
           { des_ifs; try lia.
             - rewrite URA.unit_idl. reflexivity.
             - rewrite URA.unit_id. reflexivity.
@@ -407,23 +494,30 @@ Section WSATS.
             rewrite URA.unit_id. reflexivity.
           }
       }
-      unfold wsat_auth. rewrite H3. iDestruct "AUTH" as "[AUTH NEW]".
-      unfold OwnDs_auth. rewrite H4. iDestruct "DA" as "[DA NEWD]".
-      iPoseProof (wsat_init with "[NEWD NEW]") as "NEW"; iFrame.
-      subst x. iFrame.
+      unfold wsats_auth. rewrite H3. iDestruct "AUTH" as "[AUTH NEW]".
+      rewrite H4. iDestruct "DA" as "[DA NEWD]".
+      iPoseProof (wsat_init with "[NEWD NEW]") as "NEW". iFrame.
       replace (S n - n) with 1 by lia. ss. iFrame.
-    - iIntros "[DA AUTH]". iPoseProof (IHNIN with "[DA AUTH]") as "[DA [AUTH SAT]]"; iFrame.
-      clear IHNIN. remember (S m) as y.
-      assert ((wsat_auth_black m) =
-                ((wsat_auth_black y)
+    - unfold wsats_auth in *.
+      iIntros "[DA AUTH]". iPoseProof (IHNIN with "[DA AUTH]") as "[[DA AUTH] SAT]". iFrame.
+      clear IHNIN.
+      assert ((wsats_auth_black u m) =
+                ((wsats_auth_black u (S m))
                    ⋅
-                   (maps_to_res_dep m (@Auth.black (positive ==> URA.agree (Vars m))%ra (fun (i : positive) => None))))).
-      { subst. extensionalities a. unfold wsat_auth_black, maps_to_res_dep.
-        unfold URA.add. unseal "ra". ss.
-        destruct (excluded_middle_informative (a = m)).
-        - subst a. des_ifs; try lia.
+                   (maps_to_res u (maps_to_res_dep m (@Auth.black (positive ==> URA.agree (Vars m))%ra (fun (i : positive) => None)))))).
+      { extensionalities u' m'. unfold wsats_auth_black, maps_to_res, maps_to_res_dep.
+        do 2 (unfold URA.add; unseal "ra"; ss).
+        destruct (u' =? u)%positive eqn: EQ; cycle 1.
+        { apply Pos.eqb_neq in EQ.
+          destruct (excluded_middle_informative (u' = u)); ss.
+          setoid_rewrite URA.unit_id. eauto.
+        }
+        apply Pos.eqb_eq in EQ. subst.
+        destruct (excluded_middle_informative (u=u)); ss.
+        destruct (excluded_middle_informative (m' = m)).
+        - subst. des_ifs; try lia.
           unfold eq_rect_r. ss. rewrite URA.unit_idl. reflexivity.
-        - destruct (le_dec a (S m)).
+        - destruct (le_dec m' (S m)).
           { des_ifs; try lia.
             - rewrite URA.unit_idl. reflexivity.
             - rewrite URA.unit_id. reflexivity.
@@ -432,16 +526,23 @@ Section WSATS.
             rewrite URA.unit_id. reflexivity.
           }
       }
-      assert ((OwnDs_auth_black m) =
-                ((OwnDs_auth_black y)
-                   ⋅
-                   (maps_to_res m (Auth.black (Some ∅ : Gset.t))))).
-      { subst. extensionalities a. unfold OwnDs_auth_black, maps_to_res.
-        unfold URA.add. unseal "ra". ss.
-        destruct (excluded_middle_informative (a = m)).
-        - subst a. des_ifs; try lia.
+      assert ((OwnDs_auth_black u m) =
+              ((OwnDs_auth_black u (S m))
+              ⋅
+              (maps_to_res u (maps_to_res m (Auth.black (Some ∅ : Gset.t)))))).
+      { extensionalities u' m'. unfold OwnDs_auth_black, maps_to_res.
+        do 2 (unfold URA.add; unseal "ra"; ss).
+        destruct (u' =? u)%positive eqn: EQ; cycle 1.
+        { apply Pos.eqb_neq in EQ.
+          destruct (excluded_middle_informative (u' = u)); ss.
+          setoid_rewrite URA.unit_id. eauto.
+        }
+        apply Pos.eqb_eq in EQ. subst.
+        destruct (excluded_middle_informative (u=u)); ss.
+        destruct (excluded_middle_informative (m' = m)).
+        - subst. des_ifs; try lia.
           unfold eq_rect_r. ss. rewrite URA.unit_idl. reflexivity.
-        - destruct (le_dec a (S m)).
+        - destruct (le_dec m' (S m)).
           { des_ifs; try lia.
             - rewrite URA.unit_idl. reflexivity.
             - rewrite URA.unit_id. reflexivity.
@@ -450,115 +551,111 @@ Section WSATS.
             rewrite URA.unit_id. reflexivity.
           }
       }
-      unfold wsat_auth. rewrite H3. iDestruct "AUTH" as "[AUTH NEW]".
-      unfold OwnDs_auth. rewrite H4. iDestruct "DA" as "[DA NEWD]".
-      iPoseProof (wsat_init with "[NEWD NEW]") as "NEW"; iFrame.
-      subst y. iFrame.
-      replace (S m - x) with ((m - x) + 1) by lia. rewrite seq_app.
+      rewrite H3. iDestruct "AUTH" as "[AUTH NEW]".
+      rewrite H4. iDestruct "DA" as "[DA NEWD]".
+      iPoseProof (wsat_init with "[NEWD NEW]") as "NEW". iFrame.
+      iFrame. replace (S m - n) with ((m - n) + 1) by lia. rewrite seq_app.
       iApply big_sepL_app. iFrame.
-      replace (x + (m - x)) with m by lia. ss. iFrame.
+      replace (n + (m - n)) with m by lia. ss. iFrame.
   Qed.
 
-  Lemma wsats_nin (x n : index) (NIN : x < n)
-    : wsats x ∗ ([∗ list] m ∈ (seq x (n - x)), wsat m) ⊢ wsats n.
+  Lemma wsats_nin u (n n' : level):
+    n < n' -> wsats u n ∗ ([∗ list] m ∈ (seq n (n' - n)), wsat u m) ⊢ wsats u n'.
   Proof.
-    iIntros "[SALL WSAT]". unfold wsats.
-    replace n with (x + (n - x)) by lia. rewrite seq_app; iFrame.
-    replace (x + (n - x) - x) with (n - x) by lia. iFrame.
+    iIntros (LT) "[SALL WSAT]". unfold wsats.
+    replace n' with (n + (n' - n)) at 2 by lia. rewrite seq_app. iFrame.
   Qed.
 
-  Lemma wsats_in (x0 x1 : index) :
-    x0 < x1 -> wsats x1 ⊢ wsats x0 ∗ ([∗ list] n ∈ (seq x0 (x1 - x0)), wsat n).
+  Lemma wsats_in u (n n' : level):
+    n < n' -> wsats u n' ⊢ wsats u n ∗ ([∗ list] m ∈ (seq n (n' - n)), wsat u m).
   Proof.
     iIntros (LT) "SAT". unfold wsats.
-    replace x1 with (x0 + (x1 - x0)) by lia. rewrite (seq_app _ _ 0).
+    replace n' with (n + (n' - n)) at 1 by lia. rewrite (seq_app _ _ 0).
     iPoseProof (big_sepL_app with "SAT") as "[SAT K]". iFrame.
-    ss. replace (x0 + (x1 - x0) - x0) with (x1 - x0) by lia. iFrame.
   Qed.
 
-  Lemma wsats_allocs x1 x2 :
-    x1 < x2 ->
-    OwnDs_auth x1 ∗ wsat_auth x1 ∗ wsats x1 ⊢ (OwnDs_auth x2 ∗ wsat_auth x2 ∗ wsats x2).
+  Lemma wsats_allocs u n n':
+    n < n' -> wsats_auth u n ∗ wsats u n ⊢ wsats_auth u n' ∗ wsats u n'.
   Proof.
-    iIntros (LT) "(DA & AUTH & SAT)".
-    iPoseProof ((wsat_auth_nin _ _ LT) with "[DA AUTH]") as "(DA & AUTH & NEW)"; iFrame.
-    iPoseProof ((wsats_nin _ _ LT) with "[SAT NEW]") as "SAT"; iFrame.
+    iIntros (LT) "(AUTH & SAT)".
+    iPoseProof ((wsats_auth_nin _ _ _ LT) with "AUTH") as "(AUTH & NEW)". iFrame.
+    iPoseProof ((wsats_nin _ _ _ LT) with "[SAT NEW]") as "SAT". iFrame. iFrame.
   Qed.
 
-
-  Lemma wsats_OwnI_alloc_lt_gen x n (LT : n < x) p φ
-        (INF : forall (E : index -> option (gset positive)) n,
+  Lemma wsats_OwnI_alloc_lt_gen u n n' (LT : n < n') p φ
+        (INF : forall (E : level -> option (gset positive)) n,
             match E n with
             | None => True
             | Some G => (exists i, i ∉ G /\ φ i)
             end)
-    : wsats x ⊢ #=> (∃ i, ⌜φ i⌝ ∧ OwnI n i p) ∗ (prop n p -∗ wsats x).
+    : wsats u n' ⊢ |==> (∃ i, ⌜φ i⌝ ∧ OwnI u n i p) ∗ (prop n p -∗ wsats u n').
   Proof.
     iIntros "SALL".
     iPoseProof (big_sepL_lookup_acc with "SALL") as "[WSAT K]".
-    { apply lookup_seq_lt; eauto. }
-    iPoseProof (wsat_OwnI_alloc_gen with "WSAT") as ">[RES WSAT]".
-    { apply INF. }
-    iFrame. iModIntro. iIntros "P". iFrame. iPoseProof ("WSAT" with "P") as "WSAT".
+    apply lookup_seq_lt; eauto.
+    iPoseProof (wsat_OwnI_alloc_gen with "WSAT") as ">[RES WSAT]". apply INF. iFrame.
+    iModIntro. iIntros "P". iFrame. iPoseProof ("WSAT" with "P") as "WSAT".
     iPoseProof ("K" with "WSAT") as "SALL". iFrame.
   Qed.
 
-  Lemma wsats_OwnI_alloc_lt x n (LT : n < x) p φ
-        (INF : forall (E : index -> option (gset positive)) n,
+  Lemma wsats_OwnI_alloc_lt u n n' (LT : n < n') p φ
+        (INF : forall (E : level -> option (gset positive)) n,
             match E n with
             | None => True
             | Some G => (exists i, i ∉ G /\ φ i)
             end)
-    : wsats x ∗ prop n p ⊢ #=> (∃ i, ⌜φ i⌝ ∧ OwnI n i p) ∗ wsats x.
+    : wsats u n' ∗ prop n p ⊢ |==> (∃ i, ⌜φ i⌝ ∧ OwnI u n i p) ∗ wsats u n'.
   Proof.
     iIntros "[W P]". iMod (wsats_OwnI_alloc_lt_gen with "W") as "[I W]". 1,2: eauto.
     iModIntro. iFrame. iApply "W". iFrame.
   Qed.
 
-  Lemma wsats_OwnI_alloc_ge_gen x n (GE : x <= n) p φ
-        (INF : forall (E : index -> option (gset positive)) n,
+  Lemma wsats_OwnI_alloc_ge_gen u n' n (GE : n' <= n) p φ
+        (INF : forall (E : level -> option (gset positive)) n,
             match E n with
             | None => True
             | Some G => (exists i, i ∉ G /\ φ i)
             end)
-    : OwnDs_auth x ∗ wsat_auth x ∗ wsats x ⊢
-                 #=> ((∃ i, ⌜φ i⌝ ∧ OwnI n i p)
-                         ∗ OwnDs_auth (S n) ∗ wsat_auth (S n) ∗ (prop n p -∗ wsats (S n))).
+    : wsats_auth u n' ∗ wsats u n' ⊢
+                 |==> ((∃ i, ⌜φ i⌝ ∧ OwnI u n i p)
+                         ∗ wsats_auth u (S n) ∗ (prop n p -∗ wsats u (S n))).
   Proof.
-    iIntros "(DA & AUTH & WSAT)".
-    iPoseProof ((wsats_allocs x (S n)) with "[DA AUTH WSAT]") as "[DA [AUTH WSAT]]".
-    { lia. }
-    { iFrame. }
-    iMod ((wsats_OwnI_alloc_lt_gen (S n) n) with "WSAT") as "[RES WSAT]"; eauto.
+    iIntros "(AUTH & WSAT)".
+    iPoseProof ((wsats_allocs u n' (S n)) with "[AUTH WSAT]") as "[AUTH WSAT]". lia. iFrame.
+    iMod ((wsats_OwnI_alloc_lt_gen u n (S n)) with "WSAT") as "[RES WSAT]". auto. eauto.
     iModIntro. iFrame.
   Qed.
 
-  Lemma wsats_OwnI_alloc_ge x n (GE : x <= n) p φ
-        (INF : forall (E : index -> option (gset positive)) n,
+  Lemma wsats_OwnI_alloc_ge u n' n (GE : n' <= n) p φ
+        (INF : forall (E : level -> option (gset positive)) n,
             match E n with
             | None => True
             | Some G => (exists i, i ∉ G /\ φ i)
             end)
-    : OwnDs_auth x ∗ wsat_auth x ∗ wsats x ∗ prop n p
-                 ⊢ #=> ((∃ i, ⌜φ i⌝ ∧ OwnI n i p)
-                           ∗ OwnDs_auth (S n) ∗ wsat_auth (S n) ∗ wsats (S n)).
+    : wsats_auth u n' ∗ wsats u n' ∗ prop n p
+                 ⊢ |==> ((∃ i, ⌜φ i⌝ ∧ OwnI u n i p)
+                           ∗ wsats_auth u (S n) ∗ wsats u (S n)).
   Proof.
-    iIntros "(D & A & W & P)". iMod (wsats_OwnI_alloc_ge_gen with "[D A W]") as "(I & D & A & W)".
+    iIntros "(A & W & P)". iMod (wsats_OwnI_alloc_ge_gen with "[A W]") as "(I & A & W)".
     1,2: eauto.
-    { iFrame. }
-    iModIntro. iFrame. iApply "W". iFrame.
+    iFrame. iModIntro. iFrame. iApply "W". iFrame.
   Qed.
 
-  Lemma wsat_auth_OwnI_le x n i p :
-    OwnI n i p ∗ wsat_auth x ⊢ ⌜n < x⌝.
+  Lemma wsats_auth_OwnI_le u n n' i p :
+    OwnI u n i p ∗ wsats_auth u n' ⊢ ⌜n < n'⌝.
   Proof.
-    iIntros "(I & AUTH)".
-    unfold OwnI, wsat_auth.
+    iIntros "(I & (_ & AUTH))".
+    unfold OwnI, wsats_auth.
     iCombine "AUTH I" as "AUTH".
     iPoseProof (OwnM_valid with "AUTH") as "%WF".
-    unfold wsat_auth_black, OwnI_white, maps_to_res_dep in WF.
+    unfold wsats_auth_black, OwnI_white, maps_to_res, maps_to_res_dep in WF.
     unfold URA.add in WF. unseal "ra". ss.
-    apply (pwd_lookup_wf _ n) in WF. ss. des_ifs.
+    apply (pw_lookup_wf _ u) in WF. ss.
+    unfold URA.add in WF. unseal "ra". ss.
+    apply (pwd_lookup_wf _ n) in WF. ss.
+    destruct (u =? u)%positive eqn:EQ; cycle 1.
+    { apply Pos.eqb_neq in EQ. ss. }
+    des_ifs.
     exfalso. unfold eq_rect_r in WF. rewrite <- Eqdep.EqdepTheory.eq_rect_eq in WF.
     unfold maps_to_res in WF. apply Auth.auth_included in WF. rename WF into EXTENDS.
     apply pw_extends in EXTENDS. specialize (EXTENDS i). des_ifs.
@@ -566,85 +663,98 @@ Section WSATS.
     ss. des_ifs.
   Qed.
 
-  Lemma wsats_OwnI_open x n i p :
-    n < x -> OwnI n i p ∗ wsats x ∗ OwnE n {[i]} ⊢ #=> prop n p ∗ wsats x ∗ OwnD n {[i]}.
+  Lemma wsats_OwnI_open u n n' i p:
+    n < n' -> OwnI u n i p ∗ wsats u n' ∗ OwnE u n {[i]} ⊢ |==> prop n p ∗ wsats u n' ∗ OwnD u n {[i]}.
   Proof.
     iIntros (LT) "(I & SAT & EN)".
     unfold OwnI, wsats.
     iPoseProof (big_sepL_lookup_acc with "SAT") as "[WSAT K]".
-    { apply lookup_seq_lt; eauto. }
-    ss. iMod (wsat_OwnI_open with "[I WSAT EN]") as "[P [WSAT DN]]". { iFrame. }
+    apply lookup_seq_lt; eauto.
+    ss. iMod (wsat_OwnI_open with "[I WSAT EN]") as "[P [WSAT DN]]". iFrame.
     iPoseProof ("K" with "WSAT") as "SAT".
     iModIntro. iFrame.
   Qed.
 
-  Lemma wsats_OwnI_close x n i p :
-    n < x -> OwnI n i p ∗ wsats x ∗ prop n p ∗ OwnD n {[i]} ⊢ #=> wsats x ∗ OwnE n {[i]}.
+  Lemma wsats_OwnI_close u n n' i p:
+    n < n' -> OwnI u n i p ∗ wsats u n' ∗ prop n p ∗ OwnD u n {[i]} ⊢ |==> wsats u n' ∗ OwnE u n {[i]}.
   Proof.
     iIntros (LT) "(I & SAT & P & DIS)".
     iPoseProof (big_sepL_lookup_acc with "SAT") as "[WSAT K]".
-    { apply lookup_seq_lt; eauto. }
-    iMod (wsat_OwnI_close with "[I WSAT P DIS]") as "[WSAT EN]". { iFrame. }
+    apply lookup_seq_lt; eauto.
+    iMod (wsat_OwnI_close with "[I WSAT P DIS]") as "[WSAT EN]". iFrame.
     iPoseProof ("K" with "WSAT") as "SAT".
     iModIntro. iFrame.
   Qed.
 
 End WSATS.
 
-Notation coPsets := (gmap index coPset).
+Notation coPsets := (gmap level coPset).
 
 Section OWNES.
 
   Context `{Σ : GRA.t}.
   Context `{@GRA.inG OwnEsRA Σ}.
 
-  Definition OwnE_auth_black (Es : coPsets) : (index ==> CoPset.t)%ra :=
-    fun n => match Es !! n with
-          | Some _ => ε
-          | None => (Some ⊤)
-          end.
+  Definition OwnE_auth_black u (Es : coPsets) : (universe ==> (level ==> CoPset.t))%ra :=
+    fun u' n =>
+      if (u' =? u)%positive
+      then
+        match Es !! n with
+        | Some _ => ε
+        | None => Some ⊤
+        end
+      else
+        (if (pos_sup u u')
+         then Some ⊤
+         else ε).
 
-  Definition OwnE_auth (Es : coPsets) := OwnM (OwnE_auth_black Es).
+  Definition OwnE_auth u (Es : coPsets) := OwnM (OwnE_auth_black u Es).
 
-  Definition OwnE_satall (Es : coPsets) := ([∗ map] n ↦ E ∈ Es, OwnE n E)%I.
+  Definition OwnE_satall u (Es : coPsets) := ([∗ map] n ↦ E ∈ Es, OwnE u n E)%I.
 
-  Definition OwnEs (Es : coPsets) := (OwnE_auth Es ∗ OwnE_satall Es)%I.
+  Definition OwnEs u (Es : coPsets) := (OwnE_auth u Es ∗ OwnE_satall u Es)%I.
 
   Definition OwnEs_top (Es : coPsets) : Prop := map_Forall (fun _ E => ⊤ ⊆ E) Es.
-  (* Definition OwnEs_top (Es : coPsets) : Prop := map_Forall (fun _ E => E = ⊤) Es. *)
 
-  Lemma OwnEs_init_wf :
-    URA.wf (OwnE_auth_black ∅).
+  Lemma OwnEs_init_wf u:
+    URA.wf (OwnE_auth_black u ∅).
   Proof.
-    ur. i. ur. des_ifs.
+    unfold OwnE_auth_black. ur. i. ur. i. des_ifs; ur; des_ifs.
   Qed.
 
-  Lemma OwnEs_init :
-    OwnM (OwnE_auth_black ∅) ⊢ OwnEs ∅.
+  Lemma OwnEs_init u:
+    OwnM (OwnE_auth_black u ∅) ⊢ OwnEs u ∅.
   Proof.
     iIntros. unfold OwnEs. iFrame. unfold OwnE_satall. ss.
   Qed.
 
-  Lemma OwnEs_has Es n E :
-    (Es !! n = Some E) -> OwnEs Es ⊢ OwnEs (<[n:=E]>Es).
+  Lemma OwnEs_has u Es n E :
+    (Es !! n = Some E) -> OwnEs u Es ⊢ OwnEs u (<[n:=E]>Es).
   Proof.
     iIntros (IN) "ES". rewrite insert_id; auto.
   Qed.
 
-  Lemma OwnEs_alloc Es n (NIN : Es !! n = None) :
-    OwnEs Es ⊢ #=> OwnEs (<[n := ⊤]>Es).
+  Lemma OwnEs_alloc u Es n:
+    (Es !! n = None) -> OwnEs u Es ⊢ |==> OwnEs u (<[n := ⊤]>Es).
   Proof.
-    iIntros "[AUTH SAT]". unfold OwnE_auth, OwnE_satall.
+    iIntros (NIN) "[AUTH SAT]". unfold OwnE_auth, OwnE_satall.
     remember (<[n := ⊤]> Es) as Es'.
     assert (URA.updatable
-              (OwnE_auth_black Es)
-              ((OwnE_auth_black Es')
-                 ⋅
-                 (maps_to_res n (Some ⊤)))).
-    { apply pointwise_updatable. i.
-      unfold OwnE_auth_black, maps_to_res. unfold URA.add. unseal "ra". ss. subst.
-      destruct (excluded_middle_informative (a = n)).
-      - subst a. des_ifs.
+              (OwnE_auth_black u Es)
+              ((OwnE_auth_black u Es')
+               ⋅
+               (@maps_to_res _ (_==>_)%ra u (maps_to_res n (Some ⊤))))).
+    { do 2 (apply pointwise_updatable; i).
+      unfold OwnE_auth_black, maps_to_res.
+      do 2 (unfold URA.add; unseal "ra"; ss).
+      destruct (a =? u)%positive eqn: EQ; cycle 1.
+      { apply Pos.eqb_neq in EQ.
+        destruct (excluded_middle_informative (a = u)); ss.
+        setoid_rewrite URA.unit_id. reflexivity. }
+      apply Pos.eqb_eq in EQ. subst.
+      destruct (excluded_middle_informative _); ss.
+      destruct (excluded_middle_informative (a0 = n)).
+      - subst. des_ifs.
         2:{ exfalso. setoid_rewrite lookup_insert in Heq0. inv Heq0. }
         rewrite URA.unit_idl. reflexivity.
       - rewrite lookup_insert_ne; auto. rewrite URA.unit_id. reflexivity.
@@ -653,28 +763,30 @@ Section OWNES.
     iModIntro. iFrame. unfold OwnE_satall. subst. iApply big_sepM_insert; auto. iFrame.
   Qed.
 
-  Lemma OwnEs_acc_in Es n E (IN : Es !! n = Some E) :
-    OwnEs Es ⊢ OwnE n E ∗ OwnEs (<[n := ∅]>Es).
+  Lemma OwnEs_acc_in u Es n E (IN : Es !! n = Some E) :
+    OwnEs u Es ⊢ OwnE u n E ∗ OwnEs u (<[n := ∅]>Es).
   Proof.
     iIntros "[AUTH SAT]". unfold OwnE_satall.
-    iAssert (OwnE n E ∗ ([∗ map] n0↦E0 ∈ delete n Es, OwnE n0 E0))%I with "[SAT]" as "[EN SAT]".
+    iAssert (OwnE u n E ∗ ([∗ map] n0↦E0 ∈ delete n Es, OwnE u n0 E0))%I with "[SAT]" as "[EN SAT]".
     { iApply big_sepM_delete; auto. }
     iPoseProof (OwnM_persistently with "EN") as "#EN2". ss.
-    iAssert ([∗ map] n0↦E0 ∈ <[n := ∅]>Es, OwnE n0 E0)%I with "[SAT]" as "SAT".
+    iAssert ([∗ map] n0↦E0 ∈ <[n := ∅]>Es, OwnE u n0 E0)%I with "[SAT]" as "SAT".
     { iApply big_sepM_insert_delete. iFrame. iApply (OwnM_extends with "EN2").
-      unfold maps_to_res. clear. exists ε. rewrite URA.unit_id. extensionalities a. des_ifs.
+      unfold maps_to_res. clear. exists ε. rewrite URA.unit_id.
+      extensionalities u' n'. des_ifs.
     }
     iFrame. iClear "EN2".
-    iApply (OwnM_extends with "AUTH"). exists ε. rewrite URA.unit_id. extensionalities a.
-    unfold OwnE_auth_black. destruct (Nat.eqb_spec a n).
+    iApply (OwnM_extends with "AUTH"). exists ε. rewrite URA.unit_id.
+    extensionalities u' n'.
+    unfold OwnE_auth_black. destruct (Nat.eqb_spec n' n).
     - subst. rewrite lookup_insert. rewrite IN. auto.
     - rewrite lookup_insert_ne; auto.
   Qed.
 
-  Lemma OwnEs_acc_new Es n (NIN : Es !! n = None) :
-    OwnEs Es ⊢ #=> OwnE n ⊤ ∗ OwnEs (<[n := ∅]>Es).
+  Lemma OwnEs_acc_new u Es n (NIN : Es !! n = None) :
+    OwnEs u Es ⊢ |==> OwnE u n ⊤ ∗ OwnEs u (<[n := ∅]>Es).
   Proof.
-    iIntros "ENS". iMod (OwnEs_alloc with "ENS") as "ENS"; eauto.
+    iIntros "ENS". iMod (OwnEs_alloc with "ENS") as "ENS". eauto.
     iModIntro.
     assert (<[n:=∅]> Es = <[n:=∅]> (<[n:=⊤]> Es)).
     { rewrite insert_insert. auto. }
@@ -683,17 +795,18 @@ Section OWNES.
     - iFrame.
   Qed.
 
-  Lemma OwnEs_union Es n E1 E2 :
-    OwnEs (<[n:=E1]> Es) ∗ OwnE n E2 ⊢ OwnEs (<[n:=E1 ∪ E2]> Es).
+  Lemma OwnEs_union u Es n E1 E2 :
+    OwnEs u (<[n:=E1]> Es) ∗ OwnE u n E2 ⊢ OwnEs u (<[n:=E1 ∪ E2]> Es).
   Proof.
     iIntros "[[AUTH SAT] EN]". unfold OwnEs. iSplitL "AUTH".
-    { iApply (OwnM_extends with "AUTH"). exists ε. rewrite URA.unit_id. extensionalities a.
-      unfold OwnE_auth_black. destruct (Nat.eqb_spec a n).
+    { iApply (OwnM_extends with "AUTH"). exists ε. rewrite URA.unit_id.
+      extensionalities u' n'.
+      unfold OwnE_auth_black. destruct (Nat.eqb_spec n' n).
       - subst. rewrite ! lookup_insert. auto.
       - rewrite ! lookup_insert_ne; auto.
     }
     iApply big_sepM_insert_delete.
-    iAssert (OwnE n E1 ∗ (OwnE_satall (delete n (<[n:=E1]> Es))))%I with "[SAT]" as "[EN' SAT]".
+    iAssert (OwnE u n E1 ∗ (OwnE_satall u (delete n (<[n:=E1]> Es))))%I with "[SAT]" as "[EN' SAT]".
     { iApply big_sepM_delete.
       - apply lookup_insert.
       - iFrame.
@@ -703,23 +816,29 @@ Section OWNES.
     rewrite H0. iFrame. iApply OwnE_union. iFrame.
   Qed.
 
-  Lemma OwnEs_free Es n :
-    Es !! n = None -> OwnEs (<[n:=⊤]>Es) ⊢ #=> OwnEs Es.
+  Lemma OwnEs_free u Es n :
+    Es !! n = None -> OwnEs u (<[n:=⊤]>Es) ⊢ |==> OwnEs u Es.
   Proof.
-    iIntros (NIN) "ENS". iPoseProof (OwnEs_acc_in with "ENS") as "[EN ENS]".
-    { apply lookup_insert. }
+    iIntros (NIN) "ENS". iPoseProof (OwnEs_acc_in with "ENS") as "[EN ENS]". apply lookup_insert.
     rewrite insert_insert. unfold OwnEs. iDestruct "ENS" as "[AUTH SAT]".
     iSplitL "EN AUTH".
     - unfold OwnE_auth, OwnE. iCombine "EN AUTH" as "AUTH".
       assert (URA.updatable
-                ((@maps_to_res index CoPset.t n (Some ⊤))
-                   ⋅
-                   OwnE_auth_black (<[n:=∅]> Es))
-                (OwnE_auth_black Es)).
-      { apply pointwise_updatable. i.
-        unfold OwnE_auth_black, maps_to_res. unfold URA.add. unseal "ra". ss.
-        destruct (excluded_middle_informative (a = n)).
-        - subst a. rewrite lookup_insert. rewrite NIN.
+                ((maps_to_res u (@maps_to_res level CoPset.t n (Some ⊤)))
+                 ⋅
+                 OwnE_auth_black u (<[n:=∅]> Es))
+                (OwnE_auth_black u Es)).
+      { do 2 (apply pointwise_updatable; i).
+        unfold OwnE_auth_black, maps_to_res.
+        do 2 (unfold URA.add; unseal "ra"; ss).
+        destruct (a =? u)%positive eqn: EQ; cycle 1.
+        { apply Pos.eqb_neq in EQ.
+          destruct (excluded_middle_informative (a = u)); ss.
+          setoid_rewrite URA.unit_idl. reflexivity. }
+        apply Pos.eqb_eq in EQ. subst.
+        destruct (excluded_middle_informative _); ss.
+        destruct (excluded_middle_informative (a0 = n)).
+        - subst. rewrite lookup_insert. rewrite NIN.
           rewrite URA.unit_id. reflexivity.
         - rewrite lookup_insert_ne; auto. rewrite URA.unit_idl. reflexivity.
       }
@@ -728,42 +847,42 @@ Section OWNES.
       iPoseProof (big_sepM_insert with "SAT") as "[_ SAT]"; auto.
   Qed.
 
-  Lemma OwnEs_update_one Es n E1 E2 :
-    OwnEs (<[n:=E1]>Es) ⊢ (OwnE n E1 -∗ OwnE n E2) -∗ OwnEs (<[n:=E2]>Es).
+  Lemma OwnEs_update_one u Es n E1 E2 :
+    OwnEs u (<[n:=E1]>Es) ⊢ (OwnE u n E1 -∗ OwnE u n E2) -∗ OwnEs u (<[n:=E2]>Es).
   Proof.
     iIntros "E IMPL". iPoseProof (OwnEs_acc_in with "E") as "[E K]".
     { apply lookup_insert. }
     iPoseProof ("IMPL" with "E") as "E".
     iEval (rewrite insert_insert) in "K".
-    iPoseProof (OwnEs_union with "[E K]") as "E". { iFrame. }
+    iPoseProof (OwnEs_union with "[E K]") as "E". iFrame.
     replace (∅ ∪ E2) with E2 by set_solver.
     iFrame.
   Qed.
 
-  Lemma OwnEs_subset Es n E1 E2 :
-    (E1 ⊆ E2) -> OwnEs (<[n:=E2]>Es) ⊢ OwnEs (<[n:=E1]>Es).
+  Lemma OwnEs_subset u Es n E1 E2 :
+    (E1 ⊆ E2) -> OwnEs u (<[n:=E2]>Es) ⊢ OwnEs u (<[n:=E1]>Es).
   Proof.
     iIntros (SUB) "ES". iApply (OwnEs_update_one with "ES").
-    iIntros "E". iPoseProof (OwnE_subset with "E") as "[E1 _]"; eauto.
+    iIntros "E". iPoseProof (OwnE_subset with "E") as "[E1 _]". eauto. iFrame.
   Qed.
 
-  Lemma OwnEs_disjoint Es n E1 E2 :
-    E1 ## E2 -> OwnEs (<[n:=E1 ∪ E2]>Es) ⊢ OwnEs (<[n:=E1]>Es) ∗ OwnE n E2.
+  Lemma OwnEs_disjoint u Es n E1 E2 :
+    E1 ## E2 -> OwnEs u (<[n:=E1 ∪ E2]>Es) ⊢ OwnEs u (<[n:=E1]>Es) ∗ OwnE u n E2.
   Proof.
     iIntros (HE) "ENS". iPoseProof (OwnEs_acc_in with "ENS") as "[EN ENS]".
     { apply lookup_insert. }
-    iPoseProof ((OwnE_disjoint _ _ _ HE) with "EN") as "[EN1 EN2]".
+    iPoseProof ((OwnE_disjoint _ _ _ _ HE) with "EN") as "[EN1 EN2]".
     iFrame. rewrite insert_insert.
     iApply (OwnEs_update_one with "ENS"). iIntros. iFrame.
   Qed.
 
-  Lemma OwnEs_free_all Es :
-    OwnEs_top Es -> OwnEs Es ⊢ #=> OwnEs ∅.
+  Lemma OwnEs_free_all u Es :
+    OwnEs_top Es -> OwnEs u Es ⊢ |==> OwnEs u ∅.
   Proof.
     pattern Es. revert Es. apply map_ind.
     { iIntros (TOP) "ES". ss. }
     iIntros (? ? ? NONE IND TOP) "ES".
-    iMod (OwnEs_free with "[ES]") as "ES"; eauto.
+    iMod (OwnEs_free with "[ES]") as "ES". eauto.
     { eapply map_Forall_lookup_1 in TOP. 2: apply lookup_insert. iApply OwnEs_subset; eauto. }
     iApply IND. 2: iFrame.
     eapply map_Forall_insert_1_2; eauto.
@@ -778,8 +897,8 @@ Section OWNES.
   Definition insert_def (Es : coPsets) (n : nat) : coPsets :=
     match Es !! n with | Some E => Es | None => <[n:=⊤]> Es end.
 
-  Lemma OwnEs_lookup_def Es n :
-    OwnEs Es ⊢ #=> OwnEs (<[n := lookup_def Es n]>Es).
+  Lemma OwnEs_lookup_def u Es n :
+    OwnEs u Es ⊢ |==> OwnEs u (<[n := lookup_def Es n]>Es).
   Proof.
     iIntros "ENS". unfold lookup_def, default. des_ifs; ss.
     - rewrite insert_id; auto.
@@ -800,61 +919,60 @@ Notation "E '⪿' '(' Es ',' n ')'" := (subseteq_def Es n E) (at level 70).
 Section FANCY_UPDATE.
 
   Context `{Σ : GRA.t}.
-  Context `{Vars : index -> Type}.
+  Context `{Vars : level -> Type}.
   Context `{Invs : @IInvSet Σ Vars}.
   Context `{@GRA.inG OwnEsRA Σ}.
   Context `{@GRA.inG OwnDsRA Σ}.
   Context `{@GRA.inG (IInvSetRA Vars) Σ}.
 
-  Definition inv (n : index) (N : namespace) p :=
-    (∃ i, ⌜i ∈ (↑N : coPset)⌝ ∧ OwnI n i p)%I.
+  Definition inv u (n : level) (N : namespace) p :=
+    (∃ i, ⌜i ∈ (↑N : coPset)⌝ ∧ OwnI u n i p)%I.
 
-  Definition FUpd x (A : iProp) (Es1 Es2 : coPsets) (P : iProp) : iProp :=
-    A ∗ wsats x ∗ OwnEs Es1 -∗ #=> (A ∗ wsats x ∗ OwnEs Es2 ∗ P).
+  Definition FUpd u n (A : iProp) (Es1 Es2 : coPsets) (P : iProp) : iProp :=
+    A ∗ wsats u n ∗ OwnEs u Es1 -∗ #=> (A ∗ wsats u n ∗ OwnEs u Es2 ∗ P).
 
-
-  Lemma FUpd_mono x0 x1 A Es1 Es2 P :
-    (x0 < x1) -> FUpd x0 A Es1 Es2 P ⊢ FUpd x1 A Es1 Es2 P.
+  Lemma FUpd_mono u n n' A Es1 Es2 P :
+    (n < n') -> FUpd u n A Es1 Es2 P ⊢ FUpd u n' A Es1 Es2 P.
   Proof.
     iIntros (LT) "FUPD (A & SAT & EN)".
-    iPoseProof ((wsats_in _ _ LT) with "SAT") as "[SAT K]".
-    iMod ("FUPD" with "[A SAT EN]") as "(A & SAT & EN & P)". { iFrame. }
-    iModIntro. iFrame. iApply wsats_nin; [apply LT | iFrame].
+    iPoseProof ((wsats_in _ _ _ LT) with "SAT") as "[SAT K]".
+    iMod ("FUPD" with "[A SAT EN]") as "(A & SAT & EN & P)". iFrame.
+    iModIntro. iFrame. iApply wsats_nin. apply LT. iFrame.
   Qed.
 
-  Lemma wsats_inv_gen x A Es n N p :
-    n < x ->
-    ⊢ A ∗ wsats x ∗ OwnEs Es -∗ #=> (A ∗ (prop n p -∗ wsats x) ∗ OwnEs Es ∗ (inv n N p)).
+  Lemma wsats_inv_gen u n' A Es n N p :
+    n < n' ->
+    ⊢ A ∗ wsats u n' ∗ OwnEs u Es -∗ #=> (A ∗ (prop n p -∗ wsats u n') ∗ OwnEs u Es ∗ (inv u n N p)).
   Proof.
     iIntros (LT) "(A & WSAT & EN)".
-    iMod (wsats_OwnI_alloc_lt_gen _ _ LT p (fun i => i ∈ ↑N) with "WSAT") as "[I WSAT]".
+    iMod (wsats_OwnI_alloc_lt_gen _ _ _ LT p (fun i => i ∈ ↑N) with "WSAT") as "[I WSAT]".
     - i. des_ifs. apply iris.base_logic.lib.invariants.fresh_inv_name.
     - iFrame. auto.
   Qed.
 
-  Lemma FUpd_alloc_gen x A Es n N p :
-    n < x -> (inv n N p -∗ prop n p) ⊢ FUpd x A Es Es (inv n N p).
+  Lemma FUpd_alloc_gen u n' A Es n N p :
+    n < n' -> (inv u n N p -∗ prop n p) ⊢ FUpd u n' A Es Es (inv u n N p).
   Proof.
     iIntros (LT) "P (A & WSAT & EN)".
-    iMod (wsats_inv_gen with "[A WSAT EN]") as "(A & W & EN & #INV)". { eauto. }
-    { iSplitL "A".  { iApply "A". }  iFrame. }
+    iMod (wsats_inv_gen with "[A WSAT EN]") as "(A & W & EN & #INV)". eauto.
+    iSplitL "A". iApply "A". iFrame.
     iPoseProof ("P" with "INV") as "P". iPoseProof ("W" with "P") as "W". iModIntro. iFrame. auto.
   Qed.
 
-  Lemma FUpd_alloc x A Es n N p :
-    n < x -> prop n p ⊢ FUpd x A Es Es (inv n N p).
+  Lemma FUpd_alloc u n' A Es n N p :
+    n < n' -> prop n p ⊢ FUpd u n' A Es Es (inv u n N p).
   Proof.
-    iIntros (LT) "P". iApply FUpd_alloc_gen; eauto.
+    iIntros (LT) "P". iApply FUpd_alloc_gen. auto. iIntros. iFrame.
   Qed.
 
-  Lemma FUpd_open_aux x A Es n N E (LT : n < x) (INE : Es !! n = Some E) (IN : ↑N ⊆ E) p :
-    inv n N p ⊢
-        FUpd x A Es (<[n := E∖↑N]> Es)
-        ((prop n p) ∗ ((prop n p) -∗ FUpd x A (<[n := E∖↑N]> Es) Es emp)).
+  Lemma FUpd_open_aux u n' A Es n N E (LT : n < n') (INE : Es !! n = Some E) (IN : ↑N ⊆ E) p :
+    inv u n N p ⊢
+        FUpd u n' A Es (<[n := E∖↑N]> Es)
+        ((prop n p) ∗ ((prop n p) -∗ FUpd u n' A (<[n := E∖↑N]> Es) Es emp)).
   Proof.
     iIntros "[% (%iN & #HI)] (A & WSAT & ENS)".
-    iPoseProof ((OwnEs_acc_in _ _ _ INE) with "ENS") as "[EN ENS]".
-    iAssert (OwnE n (E ∖ ↑N) ∗ OwnE n (↑N ∖ {[i]}) ∗ OwnE n {[i]})%I with "[EN]" as "(EN1 & EN2 & EN3)".
+    iPoseProof ((OwnEs_acc_in _ _ _ _ INE) with "ENS") as "[EN ENS]".
+    iAssert (OwnE u n (E ∖ ↑N) ∗ OwnE u n (↑N ∖ {[i]}) ∗ OwnE u n {[i]})%I with "[EN]" as "(EN1 & EN2 & EN3)".
     { iApply bi.sep_mono_r.
       { apply OwnE_disjoint. set_solver. }
       iApply OwnE_disjoint.
@@ -865,81 +983,80 @@ Section FANCY_UPDATE.
         + rewrite <- union_difference_singleton_L; ss. eapply union_difference_L; ss.
         + rewrite union_comm_L. f_equal. rewrite union_comm_L. ss.
     }
-    iMod (wsats_OwnI_open x n i p LT with "[HI WSAT EN3]") as "(P & WSAT & DIS)".
+    iMod (wsats_OwnI_open _ _ _ i p LT with "[HI WSAT EN3]") as "(P & WSAT & DIS)".
     { iFrame. auto. }
-    iModIntro. iFrame. iPoseProof (OwnEs_union with "[ENS EN1]") as "ENS". { iFrame. }
+    iModIntro. iFrame. iPoseProof (OwnEs_union with "[ENS EN1]") as "ENS". iFrame.
     replace (∅ ∪ E ∖ ↑N) with (E ∖ ↑N). 2: set_solver.
     iFrame. iIntros "P (A & WSAT & EN1)".
-    iMod (wsats_OwnI_close x n i p LT with "[HI WSAT P DIS]") as "(WSAT & EN3)".
+    iMod (wsats_OwnI_close _ _ _ i p LT with "[HI WSAT P DIS]") as "(WSAT & EN3)".
     { iFrame. auto. }
     iModIntro. iFrame. iSplit; auto.
-    iPoseProof (OwnE_union with "[EN2 EN3]") as "EN2". { iFrame. }
+    iPoseProof (OwnE_union with "[EN2 EN3]") as "EN2". iFrame.
     rewrite <- union_difference_singleton_L; ss.
-    iPoseProof (OwnEs_union with "[EN1 EN2]") as "ENS". { iFrame. }
-    rewrite insert_id. { iFrame. } rewrite INE. f_equal.
+    iPoseProof (OwnEs_union with "[EN1 EN2]") as "ENS". iFrame.
+    rewrite insert_id. iFrame. rewrite INE. f_equal.
     rewrite difference_union_L. set_solver.
   Qed.
 
-  Lemma FUpd_open x A Es n N (LT : n < x) (IN : (↑N) ⪿ (Es, n)) p :
-    inv n N p ⊢
-        FUpd x A Es
+  Lemma FUpd_open u n' A Es n N (LT : n < n') (IN : (↑N) ⪿ (Es, n)) p :
+    inv u n N p ⊢
+        FUpd u n' A Es
         (<[n := (Es !? n)∖↑N]> Es)
-        ((prop n p) ∗ ((prop n p) -∗ FUpd x A (<[n := (Es !? n)∖↑N]> Es) Es emp)).
+        ((prop n p) ∗ ((prop n p) -∗ FUpd u n' A (<[n := (Es !? n)∖↑N]> Es) Es emp)).
   Proof.
     iIntros "[% (%iN & #HI)] (A & WSAT & ENS)".
     unfold lookup_def, subseteq_def in *. destruct (Es !! n) eqn:CASES; ss.
-    - iApply FUpd_open_aux; auto. { unfold inv; auto. } iFrame.
+    - iApply FUpd_open_aux; auto. unfold inv; auto. iFrame.
     - iAssert (
-          (#=> (A ∗ (wsats x ∗ (OwnEs (<[n:=⊤ ∖ ↑N]> Es) ∗ (prop n p ∗ (prop n p -∗ FUpd x A (<[n:=⊤ ∖ ↑N]> Es) (<[n:=⊤]>Es) emp))))))
+          (#=> (A ∗ (wsats u n' ∗ (OwnEs u (<[n:=⊤ ∖ ↑N]> Es) ∗ (prop n p ∗ (prop n p -∗ FUpd u n' A (<[n:=⊤ ∖ ↑N]> Es) (<[n:=⊤]>Es) emp))))))
             -∗
-            #=> (A ∗ (wsats x ∗ (OwnEs (<[n:=⊤ ∖ ↑N]> Es) ∗ (prop n p ∗ (prop n p -∗ FUpd x A (<[n:=⊤ ∖ ↑N]> Es) Es emp))))))%I as "K".
+            #=> (A ∗ (wsats u n' ∗ (OwnEs u (<[n:=⊤ ∖ ↑N]> Es) ∗ (prop n p ∗ (prop n p -∗ FUpd u n' A (<[n:=⊤ ∖ ↑N]> Es) Es emp))))))%I as "K".
       { iIntros ">[A [SAT [ENS [P K]]]]". iModIntro. iFrame. iIntros "P".
         iPoseProof ("K" with "P") as "K". iIntros "[A [SAT ENS]]".
-        iPoseProof ("K" with "[A SAT ENS]") as ">[A [SAT [ENS _]]]". { iFrame. }
-        iMod (OwnEs_free with "ENS") as "ENS"; eauto.
+        iPoseProof ("K" with "[A SAT ENS]") as ">[A [SAT [ENS _]]]". iFrame.
+        iMod (OwnEs_free with "ENS") as "ENS". auto.
         iModIntro. iFrame.
       }
       iApply "K". iClear "K".
-      iMod (OwnEs_alloc _ _ CASES with "ENS") as "ENS". remember (<[n:=⊤]> Es) as Es'.
+      iMod (OwnEs_alloc _ _ _ CASES with "ENS") as "ENS". remember (<[n:=⊤]> Es) as Es'.
       replace (<[n:=⊤ ∖ ↑N]> Es) with (<[n:=⊤ ∖ ↑N]> Es').
       2:{ subst. rewrite insert_insert. auto. }
       iApply FUpd_open_aux; auto.
       { subst. apply lookup_insert. }
-      { unfold inv; auto. }
-      { iFrame. }
+      unfold inv; auto. iFrame.
   Qed.
 
-  Lemma FUpd_intro x A Es P :
-    #=> P ⊢ FUpd x A Es Es P.
+  Lemma FUpd_intro u n A Es P :
+    #=> P ⊢ FUpd u n A Es Es P.
   Proof.
     iIntros "P H". iMod "P". iModIntro. iFrame. iFrame.
   Qed.
 
-  Lemma FUpd_mask_frame_gen x A Es1 Es2 n E P :
+  Lemma FUpd_mask_frame_gen u n' A Es1 Es2 n E P :
     (Es1 !? n) ## E ->
-    FUpd x A Es1 Es2 P ⊢
-         FUpd x A (<[n := (Es1 !? n) ∪ E]>Es1) (<[n := (Es2 !? n) ∪ E]>Es2) P.
+    FUpd u n' A Es1 Es2 P ⊢
+         FUpd u n' A (<[n := (Es1 !? n) ∪ E]>Es1) (<[n := (Es2 !? n) ∪ E]>Es2) P.
   Proof.
     rewrite /FUpd. iIntros (D) "H (A & WSAT & ENS)".
-    iPoseProof ((OwnEs_acc_in _ n) with "ENS") as "[EN ENS]". { apply lookup_insert. }
-    iPoseProof (OwnE_disjoint _ _ _ D with "EN") as "[EN1 EN]".
-    iPoseProof (OwnEs_union with "[ENS EN1]") as "ENS". { iFrame. }
+    iPoseProof ((OwnEs_acc_in _ _ n) with "ENS") as "[EN ENS]". apply lookup_insert.
+    iPoseProof (OwnE_disjoint _ _ _ _ D with "EN") as "[EN1 EN]".
+    iPoseProof (OwnEs_union with "[ENS EN1]") as "ENS". iFrame.
     replace (∅ ∪ lookup_def Es1 n) with (lookup_def Es1 n) by set_solver.
     destruct (coPset_equiv_dec E ∅); cycle 1.
     { unfold lookup_def, default in D. des_ifs; ss.
       2:{ exfalso. set_solver. }
       rewrite insert_insert. rewrite (insert_id Es1).
       2:{ unfold lookup_def, default. rewrite Heq. ss. }
-      iPoseProof ("H" with "[A WSAT ENS]") as ">(A & WSAT & ENS2 & P)". { iFrame. }
+      iPoseProof ("H" with "[A WSAT ENS]") as ">(A & WSAT & ENS2 & P)". iFrame.
       destruct (Es2 !! n) eqn:CASES.
-      2:{ iMod ((OwnEs_acc_new _ _ CASES) with "ENS2") as "[EN2 _]".
-          iPoseProof (OwnE_exploit with "[EN EN2]") as "%DIS". { iFrame. }
+      2:{ iMod ((OwnEs_acc_new _ _ _ CASES) with "ENS2") as "[EN2 _]".
+          iPoseProof (OwnE_exploit with "[EN EN2]") as "%DIS". iFrame.
           set_solver.
       }
       unfold lookup_def. rewrite CASES. ss.
-      iPoseProof ((OwnEs_acc_in _ _ _ CASES) with "ENS2") as "[EN2 ENS]".
-      iPoseProof (OwnE_union with "[EN EN2]") as "EN". { iFrame. }
-      iPoseProof (OwnEs_union with "[ENS EN]") as "ENS". { iFrame. }
+      iPoseProof ((OwnEs_acc_in _ _ _ _ CASES) with "ENS2") as "[EN2 ENS]".
+      iPoseProof (OwnE_union with "[EN EN2]") as "EN". iFrame.
+      iPoseProof (OwnEs_union with "[ENS EN]") as "ENS". iFrame.
       replace (∅ ∪ (c0 ∪ E)) with (c0 ∪ E) by set_solver.
       iModIntro. iFrame.
     }
@@ -949,20 +1066,20 @@ Section FANCY_UPDATE.
       destruct (Es1 !! n) eqn:CASES.
       - rewrite (insert_id Es1).
         2:{ unfold lookup_def, default. rewrite CASES. ss. }
-        iPoseProof ("H" with "[A WSAT ENS]") as ">(A & WSAT & ENS2 & P)". { iFrame. }
+        iPoseProof ("H" with "[A WSAT ENS]") as ">(A & WSAT & ENS2 & P)". iFrame.
         iMod (OwnEs_lookup_def with "ENS2") as "ENS2". iModIntro. iFrame.
       - replace (lookup_def Es1 n) with (⊤ : coPset).
         2:{ unfold lookup_def, default. rewrite CASES. ss. }
-        iMod ((OwnEs_free _ _ CASES) with "ENS") as "ENS".
-        iPoseProof ("H" with "[A WSAT ENS]") as ">(A & WSAT & ENS2 & P)". { iFrame. }
+        iMod ((OwnEs_free _ _ _ CASES) with "ENS") as "ENS".
+        iPoseProof ("H" with "[A WSAT ENS]") as ">(A & WSAT & ENS2 & P)". iFrame.
         iMod (OwnEs_lookup_def with "ENS2") as "ENS2". iModIntro. iFrame.
     }
   Qed.
 
-  Lemma FUpd_mask_frame x A Es1 Es2 n E1 E2 E P :
+  Lemma FUpd_mask_frame u n' A Es1 Es2 n E1 E2 E P :
     E1 ## E ->
-    FUpd x A (<[n:=E1]>Es1) (<[n:=E2]>Es2) P ⊢
-         FUpd x A (<[n :=E1 ∪ E]>Es1) (<[n :=E2 ∪ E]>Es2) P.
+    FUpd u n' A (<[n:=E1]>Es1) (<[n:=E2]>Es2) P ⊢
+         FUpd u n' A (<[n :=E1 ∪ E]>Es1) (<[n :=E2 ∪ E]>Es2) P.
   Proof.
     iIntros (D) "FUPD".
     iPoseProof (FUpd_mask_frame_gen with "FUPD") as "FUPD".
@@ -970,13 +1087,13 @@ Section FANCY_UPDATE.
     unfold lookup_def. rewrite ! lookup_insert. ss. rewrite ! insert_insert. auto.
   Qed.
 
-  Lemma FUpd_intro_mask x A Es1 Es2 Es3 n E1 E2 P :
+  Lemma FUpd_intro_mask u n' A Es1 Es2 Es3 n E1 E2 P :
     E2 ⊆ E1 ->
-    FUpd x A (<[n:=E1]>Es1) (<[n:=E1]>Es2) P ⊢
-         FUpd x A (<[n:=E1]>Es1) (<[n:=E2]>Es2) (FUpd x A (<[n:=E2]>Es3) (<[n:=E1]>Es3) P).
+    FUpd u n' A (<[n:=E1]>Es1) (<[n:=E1]>Es2) P ⊢
+         FUpd u n' A (<[n:=E1]>Es1) (<[n:=E2]>Es2) (FUpd u n' A (<[n:=E2]>Es3) (<[n:=E1]>Es3) P).
   Proof.
     rewrite /FUpd. iIntros (HE) "H (A & WSAT & ENS)".
-    iPoseProof ("H" with "[A WSAT ENS]") as ">(A & WSAT & ENS & P)". { iFrame. }
+    iPoseProof ("H" with "[A WSAT ENS]") as ">(A & WSAT & ENS & P)". iFrame.
     iModIntro.
     rewrite (union_difference_L _ _ HE).
     iPoseProof (OwnEs_disjoint with "ENS") as "[ENS EN]".
@@ -985,94 +1102,93 @@ Section FANCY_UPDATE.
     iApply OwnEs_union. iFrame.
   Qed.
 
-  Lemma FUpd_mask_mono x A Es1 Es2 n E1 E2 P :
+  Lemma FUpd_mask_mono u n' A Es1 Es2 n E1 E2 P :
     E1 ⊆ E2 ->
-    FUpd x A (<[n:=E1]>Es1) (<[n:=E1]>Es2) P ⊢ FUpd x A (<[n:=E2]>Es1) (<[n:=E2]>Es2) P.
+    FUpd u n' A (<[n:=E1]>Es1) (<[n:=E1]>Es2) P ⊢ FUpd u n' A (<[n:=E2]>Es1) (<[n:=E2]>Es2) P.
   Proof.
     i. replace E2 with (E1 ∪ E2 ∖ E1).
     - eapply FUpd_mask_frame. set_solver.
     - symmetry. eapply leibniz_equiv. eapply union_difference. ss.
   Qed.
 
-  Global Instance from_modal_FUpd x A Es P :
-    FromModal True modality_id (FUpd x A Es Es P) (FUpd x A Es Es P) P.
+  Global Instance from_modal_FUpd u n A Es P :
+    FromModal True modality_id (FUpd u n A Es Es P) (FUpd u n A Es Es P) P.
   Proof.
     rewrite /FromModal /= /FUpd. iIntros. iModIntro. iFrame. iFrame.
   Qed.
 
-  Global Instance from_modal_FUpd_alloc x A Es n P :
-    FromModal (Es !! n = None) modality_id P (FUpd x A Es (<[n:=⊤]>Es) P) P.
+  Global Instance from_modal_FUpd_alloc u n' A Es n P :
+    FromModal (Es !! n = None) modality_id P (FUpd u n' A Es (<[n:=⊤]>Es) P) P.
   Proof.
     rewrite /FromModal /FUpd. ss.
     iIntros (HE) "P (A & WSAT & EN)".
-    iMod (OwnEs_alloc with "EN") as "EN"; eauto. iModIntro. iFrame.
+    iMod (OwnEs_alloc with "EN") as "EN". eauto. iModIntro. iFrame.
   Qed.
 
-  Global Instance from_modal_FUpd_free x A Es n P :
-    FromModal (Es !! n = None) modality_id P (FUpd x A (<[n:=⊤]>Es) Es P) P.
+  Global Instance from_modal_FUpd_free u n' A Es n P :
+    FromModal (Es !! n = None) modality_id P (FUpd u n' A (<[n:=⊤]>Es) Es P) P.
   Proof.
     rewrite /FromModal /FUpd. ss.
     iIntros (HE) "P (A & WSAT & EN)".
-    iMod (OwnEs_free with "EN") as "EN"; eauto. iModIntro. iFrame.
+    iMod (OwnEs_free with "EN") as "EN". eauto. iModIntro. iFrame.
   Qed.
 
-  Global Instance from_modal_FUpd_general x A Es n E1 E2 P :
-    FromModal (E2 ⊆ E1) modality_id P (FUpd x A (<[n:=E1]>Es) (<[n:=E2]>Es) P) P.
+  Global Instance from_modal_FUpd_general u n' A Es n E1 E2 P :
+    FromModal (E2 ⊆ E1) modality_id P (FUpd u n' A (<[n:=E1]>Es) (<[n:=E2]>Es) P) P.
   Proof.
     rewrite /FromModal /FUpd. ss.
     iIntros (HE) "P (A & WSAT & EN)". iModIntro. iFrame.
-    iPoseProof (OwnEs_acc_in with "EN") as "[EN ENS]". { apply lookup_insert. }
-    iPoseProof ((OwnE_subset _ _ _ HE) with "EN") as "[EN1 _]".
-    iPoseProof (OwnEs_union with "[ENS EN1]") as "ENS". { iFrame. }
-    rewrite insert_insert.
+    iPoseProof (OwnEs_acc_in with "EN") as "[EN ENS]". apply lookup_insert.
+    iPoseProof ((OwnE_subset _ _ _ _ HE) with "EN") as "[EN1 _]".
+    iPoseProof (OwnEs_union with "[ENS EN1]") as "ENS". iFrame. rewrite insert_insert.
     replace (∅ ∪ E2) with E2 by set_solver. iFrame.
   Qed.
 
-  Global Instance from_modal_FUpd_wrong_mask x A Es1 Es2 P :
+  Global Instance from_modal_FUpd_wrong_mask u n A Es1 Es2 P :
     FromModal (pm_error "Only non-mask-changing update modalities can be introduced directly.
 Use [FUpd_mask_frame] and [FUpd_intro_mask]")
-              modality_id (FUpd x A Es1 Es2 P) (FUpd x A Es1 Es2 P) P | 100.
+              modality_id (FUpd u n A Es1 Es2 P) (FUpd u n A Es1 Es2 P) P | 100.
   Proof.
     intros [].
   Qed.
 
-  Global Instance elim_modal_bupd_FUpd p x A Es1 Es2 P Q :
-    ElimModal True p false (#=> P) P (FUpd x A Es1 Es2 Q) (FUpd x A Es1 Es2 Q) | 10.
+  Global Instance elim_modal_bupd_FUpd p u n A Es1 Es2 P Q :
+    ElimModal True p false (|==> P) P (FUpd u n A Es1 Es2 Q) (FUpd u n A Es1 Es2 Q) | 10.
   Proof.
     rewrite /ElimModal bi.intuitionistically_if_elim /FUpd.
     iIntros (_) "[P K] I". iMod "P". iApply ("K" with "P"). iFrame.
   Qed.
 
-  Global Instance elim_modal_FUpd_FUpd p n x A Es1 Es2 Es3 P Q :
-    ElimModal (n <= x) p false (FUpd n A Es1 Es2 P) P (FUpd x A Es1 Es3 Q) (FUpd x A Es2 Es3 Q).
+  Global Instance elim_modal_FUpd_FUpd u p n n' A Es1 Es2 Es3 P Q :
+    ElimModal (n <= n') p false (FUpd u n A Es1 Es2 P) P (FUpd u n' A Es1 Es3 Q) (FUpd u n' A Es2 Es3 Q).
   Proof.
     rewrite /ElimModal bi.intuitionistically_if_elim.
     iIntros (LT) "[P K] I". inv LT.
     - rewrite /FUpd.
       iMod ("P" with "I") as "(A & WSAT & EN & P)". iApply ("K" with "P"). iFrame.
-    - iPoseProof (FUpd_mono n (S m) with "P") as "P". { lia. }
+    - iPoseProof (FUpd_mono _ n (S m) with "P") as "P". lia.
       rewrite /FUpd.
       iMod ("P" with "I") as "(A & WSAT & EN & P)". iApply ("K" with "P"). iFrame.
   Qed.
 
-  Global Instance elim_modal_FUpd_FUpd_general p x A Es0 Es1 Es2 n E0 E1 E2 E3 P Q :
+  Global Instance elim_modal_FUpd_FUpd_general p u n' A Es0 Es1 Es2 n E0 E1 E2 E3 P Q :
     ElimModal (E0 ⊆ E2) p false
-              (FUpd x A (<[n:=E0]>Es0) (<[n:=E1]>Es1) P)
+              (FUpd u n' A (<[n:=E0]>Es0) (<[n:=E1]>Es1) P)
               P
-              (FUpd x A (<[n:=E2]>Es0) (<[n:=E3]>Es2) Q)
-              (FUpd x A (<[n:=(E1 ∪ (E2 ∖ E0))]>Es1) (<[n:=E3]>Es2) Q) | 10.
+              (FUpd u n' A (<[n:=E2]>Es0) (<[n:=E3]>Es2) Q)
+              (FUpd u n' A (<[n:=(E1 ∪ (E2 ∖ E0))]>Es1) (<[n:=E3]>Es2) Q) | 10.
   Proof.
     rewrite /ElimModal bi.intuitionistically_if_elim. ss.
     iIntros (HE) "[M K]".
-    iPoseProof (FUpd_mask_frame _ _ _ _ _ _ _ (E2 ∖ E0) with "M") as "M".
+    iPoseProof (FUpd_mask_frame _ _ _ _ _ _ _ _ (E2 ∖ E0) with "M") as "M".
     { set_solver. }
     replace (E0 ∪ E2 ∖ E0) with E2 by (eapply union_difference_L; ss).
     iMod "M". iPoseProof ("K" with "M") as "M". iFrame.
   Qed.
 
   Global Instance elim_acc_FUpd
-         {X : Type} i A Es1 Es2 Es (α β : X -> iProp) (mγ : X -> option iProp) (Q : iProp) :
-    ElimAcc True (FUpd i A Es1 Es2) (FUpd i A Es2 Es1) α β mγ (FUpd i A Es1 Es Q) (fun x : X => ((FUpd i A Es2 Es2 (β x)) ∗ (mγ x -∗? FUpd i A Es1 Es Q))%I).
+         {X : Type} u i A Es1 Es2 Es (α β : X -> iProp) (mγ : X -> option iProp) (Q : iProp) :
+    ElimAcc True (FUpd u i A Es1 Es2) (FUpd u i A Es2 Es1) α β mγ (FUpd u i A Es1 Es Q) (fun x : X => ((FUpd u i A Es2 Es2 (β x)) ∗ (mγ x -∗? FUpd u i A Es1 Es Q))%I).
   Proof.
     iIntros (_) "Hinner >[% [Hα Hclose]]".
     iPoseProof ("Hinner" with "Hα") as "[>Hβ Hfin]".
@@ -1080,19 +1196,19 @@ Use [FUpd_mask_frame] and [FUpd_intro_mask]")
     iApply "Hfin". iFrame.
   Qed.
 
-  Global Instance into_acc_FUpd_inv x A Es n N p :
-    IntoAcc (inv n N p) (n < x /\ (↑N) ⪿ (Es, n)) True
-            (FUpd x A Es (<[n := Es !? n ∖ ↑N]>Es))
-            (FUpd x A (<[n := Es !? n ∖ ↑N]>Es) Es)
+  Global Instance into_acc_FUpd_inv u n' A Es n N p :
+    IntoAcc (inv u n N p) (n < n' /\ (↑N) ⪿ (Es, n)) True
+            (FUpd u n' A Es (<[n := Es !? n ∖ ↑N]>Es))
+            (FUpd u n' A (<[n := Es !? n ∖ ↑N]>Es) Es)
             (fun _ : () => prop n p) (fun _ : () => prop n p) (fun _ : () => None).
   Proof.
     rewrite /IntoAcc. iIntros ((LT & iE)) "INV _". rewrite /accessor.
-    iPoseProof (FUpd_open _ _ _ _ _ LT iE with "INV") as ">[open close]".
+    iPoseProof (FUpd_open _ _ _ _ _ _ LT iE with "INV") as ">[open close]".
     iModIntro. iExists tt. iFrame.
   Qed.
 
-  Global Instance elim_modal_iupd_FUpd p x A Es1 Es2 P Q :
-    ElimModal True p false (#=(A)=> P) P (FUpd x A Es1 Es2 Q) (FUpd x A Es1 Es2 Q) | 10.
+  Global Instance elim_modal_iupd_FUpd p u n A Es1 Es2 P Q :
+    ElimModal True p false (#=(A)=> P) P (FUpd u n A Es1 Es2 Q) (FUpd u n A Es1 Es2 Q) | 10.
   Proof.
     rewrite /ElimModal bi.intuitionistically_if_elim /FUpd.
     iIntros (_) "[P K] [A I]".
